Add soundness proof

doc/coq/simple/Equiv.v
@@ -1,4 +1,5 @@
-From Simple Require Import Concrete.
+From Simple Require Export Abstract.
+From Simple Require Export Concrete.
 
 Ltac lebt x :=
   apply leb_trans with (t' := x);
@@ -231,10 +232,9 @@ Lemma time_bound_tick `{time T} :
   forall C m t x v
          (BOUNDv : time_bound_v v t)
          (BOUNDm : time_bound_m m t),
-  let t' := tick C m t x v in
-  time_bound_m (t !-> v; m) t'.
+  time_bound_m (t !-> v; m) (tick C m t x v).
 Proof.
-  intros. subst t'.
+  intros.
   unfold time_bound_v in *.
   unfold time_bound_m in *. des_hyp.
   unfold time_bound_C in *.
@@ -503,18 +503,78 @@ Proof.
   induction fuel; intros; destruct m; simpl in *; eauto;
   try (inversion GE; fail).
   assert (List.length m <= fuel). { nia. }
-  repeat des_goal; repeat des_hyp; clarify; eauto.
-  - apply IHfuel. pose proof (remove_t_dec_len m t). nia.
-  - apply IHfuel. pose proof (remove_t_dec_len m t). nia.
-  - apply IHfuel. pose proof (reach_m_step_dec_len m init).
+  repeat des_goal; repeat des_hyp; clarify; eauto; apply IHfuel;
+  match goal with
+  | _ => pose proof (remove_t_dec_len m t); nia
+  | _ => idtac
+  end.
+  - pose proof (reach_m_step_dec_len m init).
     repeat des_hyp; ss; clarify.
     rewrite Nat.eqb_neq in *. nia.
+Qed.
+
+Lemma relax_fuel `{Eq T} :
+  forall fuel fuel' (LE : fuel' <= fuel) init m reached
+    (EV : reach_m_aux init m fuel' = Some reached),
+  reach_m_aux init m fuel = Some reached.
+Proof.
+  induction fuel;
+  ii; inv LE; ss; repeat des_goal; repeat des_hyp; clarify;
+  apply IHfuel in EV; eauto.
+  - rewrite <- EV. symmetry.
+    eapply IHfuel; eauto.
+    destruct fuel'; ss; repeat rw; eauto.
+  - destruct fuel; ss; repeat des_hyp; clarify.
+    apply IHfuel with (fuel' := fuel); eauto.
 Qed.
 
 Lemma reach_m_some `{Eq T} :
   forall m init, exists reached, reach_m init m = Some reached.
 Proof.
   intros. unfold reach_m. apply reach_m_aux_some. eauto.
+Qed.
+
+Inductive Mpath {T} : path T -> Prop :=
+  | Mnil
+    : Mpath Pnil
+  | Mcons
+    (p : path T) (M : ID) (C : dy_ctx T) (Mp : Mpath p)
+    : Mpath (p +++ (PM M (Ctx C) Pnil))
+.
+
+Fixpoint prefixof {T} (p p' : path T) :=
+  match p, p' with
+  | Pnil, _ => True
+  | Px x ntx p, Px x' ntx' p' =>
+    x = x' /\ ntx = ntx' /\ prefixof p p'
+  | PM M nCM p, PM M' nCM' p' =>
+    M = M' /\ nCM = nCM' /\ prefixof p p'
+  | Pv v nCv p, Pv v' nCv' p' =>
+    v = v' /\ nCv = nCv' /\ prefixof p p'
+  | _, _ => False
+  end.
+
+Lemma prefixof_app {T} :
+  forall (p a b : path T),
+    prefixof p (a +++ b) <->
+      prefixof p a \/ (exists p', p = a +++ p' /\ prefixof p' b).
+Proof.
+  assert (forall (pfx a b : path T), (prefixof a b) -> prefixof (pfx +++ a) (pfx +++ b)).
+  { induction pfx; intros; simpl; repeat split; eauto. }
+  induction p; intros; split; intros PFX; ss;
+  match goal with
+  | |- True \/ _ => left; auto
+  | _ => repeat des_goal; repeat des_hyp; clarify; des; ss; clarify
+  end;
+  match goal with
+  | _ => rewrite IHp in *; des; clarify; eauto
+  | _ => idtac
+  end;
+  match goal with
+  | |- False \/ _ =>
+    right; eexists; split; try reflexivity; s; auto
+  | _ => repeat split; try reflexivity; rewrite <- IHp; auto
+  end.
 Qed.
 
 Lemma asame_aequiv `{Eq T} `{Eq TT} :
@@ -713,364 +773,3 @@ Definition trans_equiv_m :=
 0.
 
 Definition trans_equiv := 0.
-
-(*
-Definition equiv_aux `{Eq T} `{Eq TT}
-  (C : dy_ctx T) m (C' : dy_ctx TT) m' :=
-  match C with
-  | [||] => C' = [||]
-  | dy_binde x t C =>
-    match addr_x C' x with
-    | None => False
-    | Some t' =>
-      <|(MVal (remove_x C x)) m ≃ (MVal (remove_x C' x)) m'|> /\
-      match read m t, read m' t' with
-      | None, None => True
-      | Some v, Some v' =>
-      <|(EVal v) (remove_t m t) ≃ (EVal v') (remove_t m' t')|>
-      | _, _ => False
-      end
-    end
-  | dy_bindm M C_M C =>
-    match ctx_M C' M with
-    | None => False
-    | Some C_M' =>
-      <|(MVal (remove_M C M)) m ≃ (MVal (remove_M C' M)) m'|> /\
-      <|(MVal C_M) m ≃ (MVal C_M') m'|>
-    end
-  end.
-
-Definition equiv_alt `{Eq T} `{Eq TT}
-  (V : dy_value T) m (V' : dy_value TT) m' :=
-  match V, V' with
-  | EVal (Closure x e C), EVal (Closure x' e' C') =>
-    x = x' /\ e = e' /\ equiv_aux C m C' m'
-  | MVal C, MVal C' =>
-    equiv_aux C m C' m'
-  | _, _ => False
-  end.
-
-Lemma equiv_alt_eq `{Eq T} `{Eq TT} :
-  forall (V : dy_value T) m (V' : dy_value TT) m'
-    (EQ : equiv_alt V m V' m'),
-  equiv V m V' m'.
-Proof.
-  intros; red in EQ.
-  repeat des_hyp; clarify; try destruct EQ as [? [? EQ]]; subst.
-  - ginduction C; intros; simpl in *; clarify.
-    + exists (fun _ => Ctx ([||])). exists (fun _ => Ctx ([||])).
-      split; intros;
-      match goal with
-      | |- _ /\ _ = ?p => destruct p; simpl in *; repeat des_hyp; eauto;
-        match goal with
-        | H : _ /\ _ /\ _ |- _ =>
-          destruct H as [? [? H]]; subst; repeat split; eauto;
-          match goal with
-          | H : valid_path _ _ ?p |- _ =>
-            destruct p; simpl in *; repeat des_hyp; eauto
-          end
-        end
-      end.
-    + repeat des_hyp; unfold equiv in EQ;
-      match goal with
-      | H : _ /\ False |- _ => destruct H; contradict
-      | H : _ /\ True |- _ => destruct H as [[f [f' [EQl EQr]]] ?];
-        match goal with
-        | H : True |- _ => clear H
-        end
-      | _ =>
-        destruct EQ as [EQt EQtx];
-        destruct EQt as [ft [ft' [EQtl EQtr]]];
-        destruct EQtx as [ftx [ftx' [EQtxl EQtxr]]]
-      end.
-      all:cycle 1.
-*)
-
-(* Set Printing Implicit. *)
-(*
-Lemma sound_eval `{Conc.time CT} `{Abs.time AT} (α : CT -> AT) (PRES : preserve_tick α) :
-  forall C st e V stV (EVAL : EvalR C st e V stV)
-    abs_C abs_st
-    (SOUND : sound_cf α C st abs_C abs_st)
-    (BOUND : time_bound C st),
-  exists abs_V abs_stV,
-    sound_res α V stV abs_V abs_stV /\
-    Abs.EvalR abs_C abs_st e abs_V abs_stV.
-Proof.
-  intros C st e V stV EVAL.
-  induction EVAL; intros; simpl in *.
-  - pose proof (trans_ctx_addr α C x) as RR.
-    rewrite <- ADDR in RR. rewrite <- STATE in SOUND.
-    exists (EVal (trans_v α v)).
-    exists abs_st. destruct abs_st.
-    repeat split; try apply SOUND.
-    eapply Abs.Eval_var_e with (addr := α addr); eauto.
-    destruct SOUND as [RRC [? ?]]. rewrite <- RRC. symmetry. assumption.
-    destruct SOUND as [? [MEM ?]].
-    red in MEM. specialize (MEM (α addr) (trans_v α v)).
-    rewrite MEM. exists addr. exists v. repeat split; eauto.
-  - exists (EVal (Closure x e (trans_ctx α C))).
-    exists abs_st.
-    destruct st as [mem t]. destruct abs_st as [abs_mem abs_t].
-    repeat split; try apply SOUND.
-    destruct SOUND as [RR [? ?]]. rewrite RR.
-    apply Abs.Eval_lam.
-  - pose proof (time_bound_e C st e1 (EVal (Closure x e C_lam)) st_lam EVAL1) as BOUND1.
-    pose proof (time_bound_e C st_lam e2 (EVal arg) (ST mem t) EVAL2) as BOUND2.
-    pose proof (time_bound_e (C_lam [|dy_binde x t ([||])|])
-                             (ST (t !-> arg; mem) (tick C (ST mem t) x arg))
-                             e (EVal v) st_v EVAL3) as BOUND3.
-    specialize (BOUND1 BOUND). simpl in BOUND1.
-    destruct st as [memi ti]. destruct st_lam as [memf tf]. destruct st_v as [memv tv].
-    apply time_increase_e in EVAL1 as time_inc1.
-    apply time_increase_e in EVAL2 as time_inc2.
-    apply time_increase_e in EVAL3 as time_inc3.
-    assert (time_bound C (ST memf tf)) as B1.
-    { simpl. simpl in BOUND. destruct BOUND as [? [? ?]].
-             simpl in BOUND1. destruct BOUND1 as [? [? ?]].
-      split. eapply relax_ctx_bound. eauto. eauto.
-      split; eauto. }
-    specialize (BOUND2 B1).
-    destruct arg. destruct v.
-    assert (time_bound (C_lam [|dy_binde x t ([||])|])
-             (ST (t !-> Closure x0 e0 C0; mem) (tick C (ST mem t) x (Closure x0 e0 C0)))) as B2.
-    { simpl. simpl in BOUND. destruct BOUND as [BB1 [BB2 BB3]].
-             simpl in BOUND1. destruct BOUND1 as [BB1' [BB2' BB3']].
-             simpl in BOUND2. destruct BOUND2 as [BB1'' [BB2'' BB3'']].
-      split. rewrite plugin_ctx_bound. split.
-      eapply relax_ctx_bound. eauto. lebt t.
-      simpl. split; eauto. split. apply tick_lt. apply tick_lt.
-      apply time_bound_tick. repeat split; eauto. }
-    specialize (BOUND3 B2).
-    specialize (IHEVAL1 abs_C abs_st SOUND BOUND).
-    destruct IHEVAL1 as [abs_V' [[memf' tf'] [SOUND1 EVAL1']]].
-    assert (sound_cf α C (ST memf tf) abs_C (Abs.ST memf' tf')) as HINT.
-    { destruct SOUND1 as [? [? ?]].
-      split. destruct abs_st; apply SOUND.
-      split; assumption. }
-    specialize (IHEVAL2 abs_C (Abs.ST memf' tf') HINT B1). clear HINT.
-    destruct IHEVAL2 as [abs_V'' [[mem' t'] [SOUND2 EVAL2']]].
-    destruct abs_V' as [[x' e' C_lam'] | ?]; 
-    inversion SOUND1 as [SOUNDV1 [SOUNDm1 SOUNDt1]];
-    try (inversion SOUNDV1; fail).
-    destruct SOUND2 as [SOUNDV2 [SOUNDm2 SOUNDt2]].
-    destruct abs_V'' as [arg' | ?]; try (inversion SOUNDV2; fail).
-    assert (sound_cf α (C_lam [|dy_binde x t ([||])|])
-            (ST (t !-> Closure x0 e0 C0; mem) (tick C (ST mem t) x (Closure x0 e0 C0)))
-            (C_lam'[| dy_binde x (α t) ([||]) |])
-            (Abs.ST ((α t) !#-> arg'; mem') 
-                    (Abs.tick abs_C (Abs.ST mem' t') x arg'))) as HINT.
-    { split. rewrite plugin_trans_ctx; inversion SOUNDV1; eauto.
-      split; try apply PRES.
-      eapply trans_mem_update; eauto. inversion SOUNDV2; eauto.
-      split. destruct abs_st; apply SOUND.
-      split; eauto.
-      inversion SOUNDV2; eauto. }
-    specialize (IHEVAL3 (C_lam' [|dy_binde x (α t) ([||])|])
-                (Abs.ST ((α t) !#-> arg'; mem') 
-                    (Abs.tick abs_C (Abs.ST mem' t') x arg')) HINT B2). clear HINT.
-    destruct IHEVAL3 as [abs_V [abs_stV [SOUND3 EVAL3']]].
-    exists abs_V. exists abs_stV.
-    split; eauto. destruct abs_stV as [memv' tv']. 
-    destruct SOUND3 as [SOUNDV3 [SOUNDm3 SOUNDt3]].
-    destruct abs_V; try (inversion SOUNDV3; fail).
-    eapply Abs.Eval_app; eauto.
-    rewrite <- SOUNDt2. inversion SOUNDV1; subst; eauto.
-  - pose proof (time_bound_e C st m (MVal C_m) st_m EVAL1) as BOUND1.
-    pose proof (time_bound_e C_m st_m e v st_v EVAL2) as BOUND2.
-    specialize (BOUND1 BOUND). simpl in BOUND1. 
-    specialize (BOUND2 BOUND1). simpl in BOUND2.
-    destruct st as [memi ti]. destruct st_m as [memm tm]. destruct st_v as [memv tv].
-    apply time_increase_e in EVAL1 as time_inc1.
-    apply time_increase_e in EVAL2 as time_inc2.
-    specialize (IHEVAL1 abs_C abs_st SOUND BOUND).
-    destruct IHEVAL1 as [[? | C_m'] [[memm' tm'] [SOUND1 EVAL1']]];
-    destruct SOUND1 as [SOUNDV1 [SOUNDm1 SOUNDt1]];
-    try (inversion SOUNDV1; fail).
-    assert (sound_cf α C_m (ST memm tm) C_m' (Abs.ST memm' tm')) as HINT.
-    { split. inversion SOUNDV1; eauto. 
-      split; assumption. }
-    specialize (IHEVAL2 C_m' (Abs.ST memm' tm') HINT BOUND1). clear HINT.
-    destruct IHEVAL2 as [abs_V [[memv' tv'] [SOUND2 EVAL2']]].
-    exists abs_V. exists (Abs.ST memv' tv').
-    split. assumption.
-    eapply Abs.Eval_link; eauto.
-  - exists (MVal abs_C). exists abs_st. destruct st; destruct abs_st.
-    split; eauto. destruct SOUND as [RR [? ?]].
-    split. simpl. rewrite RR. eauto. split; assumption.
-  - exists (MVal (trans_ctx α C_M)). exists abs_st. destruct st; destruct abs_st.
-    destruct SOUND as [? [? ?]].
-    split. split; eauto.
-    eapply Abstract.Eval_var_m. erewrite trans_ctx_ctx_M; eauto.
-  - pose proof (time_bound_e C st e (EVal v) (ST mem t) EVAL1) as BOUND1.
-    pose proof (time_bound_e (C [|dy_binde x t ([||])|]) 
-                             (ST (t !-> v; mem) (tick C (ST mem t) x v)) m
-                             (MVal C_m) st_m EVAL2) as BOUND2.
-    specialize (BOUND1 BOUND). simpl in BOUND1.
-    destruct st as [memi ti]. destruct st_m as [memm tm]. destruct v.
-    apply time_increase_e in EVAL1 as time_inc1.
-    apply time_increase_e in EVAL2 as time_inc2.
-    assert (time_bound (C [|dy_binde x t ([||])|])
-            (ST (t !-> (Closure x0 e0 C0); mem) (tick C (ST mem t) x (Closure x0 e0 C0)))) as B1.
-    { simpl. simpl in BOUND. destruct BOUND as [BB1 [BB2 BB3]].
-             simpl in BOUND1. destruct BOUND1 as [BB1' [BB2' BB3']].
-      split. rewrite plugin_ctx_bound. split.
-      eapply relax_ctx_bound. eauto. lebt t.
-      simpl. split; eauto. apply tick_lt.
-      apply time_bound_tick. repeat split; eauto. }
-    specialize (BOUND2 B1).
-    specialize (IHEVAL1 abs_C abs_st SOUND BOUND).
-    destruct IHEVAL1 as [[v' | ?] [[mem' t'] [[SOUNDV1 [SOUNDm1 SOUNDt1]] EVAL1']]];
-    try (inversion SOUNDV1; fail).
-    assert (sound_cf α (C [|dy_binde x t ([||])|])
-            (ST (t !-> Closure x0 e0 C0; mem) (tick C (ST mem t) x (Closure x0 e0 C0)))
-            (abs_C [| dy_binde x (α t) ([||]) |])
-            (Abs.ST ((α t) !#-> v'; mem')
-                    (Abs.tick abs_C (Abs.ST mem' t') x v'))) as HINT.
-    { split. rewrite plugin_trans_ctx; destruct abs_st; destruct SOUND as [RR [? ?]]; rewrite RR; eauto.
-      split; try apply PRES.
-      eapply trans_mem_update; eauto. inversion SOUNDV1; eauto.
-      split. destruct abs_st; apply SOUND.
-      split; eauto.
-      inversion SOUNDV1; eauto. }
-    specialize (IHEVAL2 (abs_C [|dy_binde x (α t) ([||])|])
-                (Abs.ST
-                  (α t !#-> v'; mem')
-                  (Abs.tick abs_C (Abs.ST mem' t') x v')) HINT B1). clear HINT.
-    destruct IHEVAL2 as [abs_V [abs_stV [SOUND2 EVAL2']]].
-    exists abs_V. exists abs_stV. split; eauto.
-    destruct abs_V as [? | ?]; 
-    destruct abs_stV; destruct SOUND2 as [contra [? ?]]; try (inversion contra; fail).
-    eapply Abs.Eval_lete; eauto. rewrite <- SOUNDt1 in *. eauto.
-  - pose proof (time_bound_e C st m' (MVal C') st' EVAL1) as BOUND1.
-    pose proof (time_bound_e (C [|dy_bindm M C' ([||])|]) st' m''
-                             (MVal C'') st'' EVAL2) as BOUND2.
-    specialize (BOUND1 BOUND). simpl in BOUND1.
-    destruct st as [memi ti]. destruct st' as [memM tM]. destruct st'' as [memV tV].
-    apply time_increase_e in EVAL1 as time_inc1.
-    apply time_increase_e in EVAL2 as time_inc2.
-    assert (time_bound (C [|dy_bindm M C' ([||])|]) (ST memM tM)) as B1.
-    { simpl. simpl in BOUND. destruct BOUND as [BB1 [BB2 BB3]].
-             simpl in BOUND1. destruct BOUND1 as [BB1' [BB2' BB3']].
-      split. rewrite plugin_ctx_bound. split.
-      eapply relax_ctx_bound. eauto. eauto. simpl. split; eauto. split; eauto. }
-    specialize (BOUND2 B1).
-    specialize (IHEVAL1 abs_C abs_st SOUND BOUND).
-    destruct IHEVAL1 as [abs_C' [[memM' tM'] [[SOUNDV1 [SOUNDm1 SOUNDt1]] EVAL1']]].
-    destruct abs_C' as [? | abs_C']; try (inversion SOUNDV1; fail).
-    assert (sound_cf α (C [|dy_bindm M C' ([||])|]) (ST memM tM)
-            (abs_C [|dy_bindm M abs_C' ([||]) |]) (Abs.ST memM' tM')) as HINT.
-    { split. rewrite plugin_trans_ctx. simpl.
-      destruct abs_st; destruct SOUND as [RR [? ?]].
-      rewrite RR; inversion SOUNDV1; subst; eauto.
-      split; eauto. }
-    specialize (IHEVAL2 (abs_C [|dy_bindm M abs_C' ([||])|])
-                        (Abs.ST memM' tM') HINT B1).
-    destruct IHEVAL2 as [abs_V [[memV' tV'] [[SOUNDV2 [SOUNDm2 SOUNDt2]] EVAL2']]].
-    exists abs_V. exists (Abs.ST memV' tV').
-    split. split. eauto. split; eauto.
-    destruct abs_V as [? | abs_V]; try (inversion SOUNDV2; fail).
-    eauto.
-Qed.
-
-Lemma sound_reach `{Conc.time CT} `{Abs.time AT} (α : CT -> AT) (PRES : preserve_tick α) :
-  forall C st e C' st' e'
-         (REACH : one_reach C st e C' st' e')
-         (BOUND : time_bound C st)
-         abs_C abs_st
-         (SOUND : sound_cf α C st abs_C abs_st),
-    exists abs_C' abs_st',
-    sound_cf α C' st' abs_C' abs_st' /\
-    Abs.one_reach abs_C abs_st e abs_C' abs_st' e'.
-Proof.
-  intros.
-  rename H into ECT. rename H0 into OCT. rename H1 into T1.
-  rename H2 into EAT. rename H3 into T2.
-  destruct st as [memi ti].
-  destruct REACH.
-  - exists abs_C. exists abs_st.
-    repeat split; eauto. apply Abs.one_appl.
-  - eapply sound_eval in FN; eauto.
-    destruct FN as [abs_V [abs_stV [SOUND' EVAL]]].
-    exists abs_C. exists abs_stV.
-    destruct st_lam as [memf tf].
-    destruct abs_stV as [memf' tf']. destruct SOUND' as [SOUNDV1 [SOUNDm1 SOUNDt1]].
-    split. split. destruct abs_st; apply SOUND. split; eauto.
-    destruct abs_V as [[x' e' C_lam'] | ?]; try (inversion SOUNDV1; fail).
-    eapply Abs.one_appr; eauto.
-  - eapply sound_eval in FN as SOUND1; eauto.
-    destruct SOUND1 as [abs_V [[memf' tf'] [SOUND1 EVAL1]]].
-    apply time_bound_e in FN as BOUND1; eauto.
-    destruct st_lam as [memf tf].
-    destruct SOUND1 as [SOUNDV1 [SOUNDm1 SOUNDt1]].
-    destruct abs_V as [[x' e' C_lam'] | ?]; try (inversion SOUNDV1; fail).
-    apply time_increase_e in FN as INC1; eauto.
-    assert (time_bound C (ST memf tf)) as B1.
-    { split. eapply relax_ctx_bound; eauto. apply BOUND.
-      apply BOUND1. }
-    assert (sound_cf α C (ST memf tf) abs_C (Abs.ST memf' tf')) as HINT.
-    { split. destruct abs_st; apply SOUND.
-      split; eauto. }
-    eapply sound_eval in ARG as SOUND2; eauto. clear HINT.
-    destruct SOUND2 as [arg' [[mem' t'] [SOUND2 EVAL2]]].
-    apply time_bound_e in ARG as BOUND2; eauto.
-    apply time_increase_e in ARG as INC2; eauto.
-    destruct SOUND2 as [SOUNDV2 [SOUNDm2 SOUNDt2]].
-    destruct arg' as [arg' | ?]; try (inversion SOUNDV2; fail).
-    exists (C_lam' [| dy_binde x (α t) ([||]) |]).
-    exists (Abs.ST (α t !#-> arg'; mem') (Abs.tick abs_C (Abs.ST mem' t') x arg')).
-    split. split.
-    rewrite plugin_trans_ctx; inversion SOUNDV1; eauto.
-    split; try apply PRES.
-    destruct arg. eapply trans_mem_update; eauto. inversion SOUNDV2; eauto.
-    split. destruct abs_st; apply SOUND.
-    split; eauto.
-    inversion SOUNDV2; eauto.
-    rewrite <- SOUNDt2 in *.
-    eapply Abs.one_appbody; eauto.
-    inversion SOUNDV1; subst; eauto.
-  - exists abs_C. exists abs_st.
-    split; eauto. eapply Abs.one_linkl; eauto.
-  - eapply sound_eval in MOD; eauto.
-    destruct MOD as [abs_V [abs_stV [SOUND1 EVAL1]]].
-    destruct st_m as [memm tm]. destruct abs_stV as [memm' tm'].
-    destruct SOUND1 as [SOUNDV1 [SOUNDm1 SOUNDt1]].
-    destruct abs_V as [? | C_m']; try (inversion SOUNDV1; fail).
-    exists C_m'. exists (Abs.ST memm' tm').
-    split. split. inversion SOUNDV1; eauto.
-    split; eauto.
-    eapply Abs.one_linkr; eauto.
-  - exists abs_C. exists abs_st. split; eauto.
-    eapply Abs.one_letel.
-  - eapply sound_eval in EVALx as SOUND1; eauto.
-    destruct SOUND1 as [abs_V [[mem' t'] [SOUND1 EVAL1]]].
-    destruct SOUND1 as [SOUNDV1 [SOUNDm1 SOUNDt1]].
-    destruct abs_V as [v' | ?]; try (inversion SOUNDV1; fail).
-    apply time_bound_e in EVALx; eauto.
-    exists (abs_C [| dy_binde x (α t) ([||]) |]).
-    exists (Abs.ST (α t !#-> v'; mem') (Abs.tick abs_C (Abs.ST mem' t') x v')).
-    split. split.
-    rewrite plugin_trans_ctx. destruct abs_st; destruct SOUND as [RR [? ?]]; rewrite RR. eauto.
-    split; try apply PRES.
-    destruct v; eapply trans_mem_update; eauto. inversion SOUNDV1; eauto.
-    split. destruct abs_st; apply SOUND.
-    split; eauto.
-    inversion SOUNDV1; eauto.
-    rewrite <- SOUNDt1 in *.
-    eapply Abs.one_leter; eauto.
-  - exists abs_C. exists abs_st.
-    split; eauto. apply Abs.one_letml.
-  - eapply sound_eval in EVALM as SOUND1; eauto.
-    destruct st_M as [memM tM].
-    destruct SOUND1 as [C_M' [[memM' tM'] [[SOUNDV1 [SOUNDm1 SOUNDt1]] EVAL1]]].
-    destruct C_M' as [? | C_M']; try (inversion SOUNDV1; fail).
-    eapply time_increase_e in EVALM as INC1; eauto.
-    eapply time_bound_e in EVALM as BOUND1; eauto.
-    exists (abs_C [|dy_bindm M C_M' ([||])|]).
-    exists (Abs.ST memM' tM').
-    split. split. rewrite plugin_trans_ctx.
-    destruct abs_st; destruct SOUND as [RR [? ?]]; rewrite RR; inversion SOUNDV1; eauto.
-    split; eauto.
-    eapply Abs.one_letmr. eauto.
-Qed.
-*)
