doc/coq/simple/Sound.v
@@ -1,0 +1,95 @@
+From Simple Require Export Equiv.
+
+Module Abs := Abstract.
+Module Conc := Concrete.
+
+Generalizable Variables CT AT.
+
+Definition preserve_tick `{Conc.time CT} `{Abs.time AT} (α : CT -> AT) :=
+  forall C m t x v,
+  let abs_C := trans_C α C in
+  let abs_m := trans_m α m in
+  let abs_t := α t in
+  let abs_v := trans_v α v in
+  α (Conc.tick C m t x v) = 
+    Abs.tick abs_C abs_m abs_t x abs_v.
+
+Lemma sound_eval `{Conc.time CT} `{Abs.time AT} (α : CT -> AT) (PRES : preserve_tick α) :
+  forall e C m t ρ (EVAL : {|(Cf e C m t) ~> ρ|})
+    (BOUND : time_bound_ρ (Cf e C m t)),
+  let abs_C := trans_C α C in
+  let abs_m := trans_m α m in
+  let abs_t := α t in
+  {|(Cf e abs_C abs_m abs_t) ~#> (trans_ρ α ρ)|}.
+Proof.
+  intros. remember (Cf e C m t) as cf.
+  ginduction EVAL; ii;
+  repeat match goal with
+  | H : {|(Rs _ _ _) ~> _|} |- _ => inversion H
+  | x := _ |- _ => subst x
+  end; clarify;
+  try match goal with
+  | ADDR : addr_x ?C ?x = Some ?addr,
+    ACCESS : read ?m ?t = Some ?v |- _ =>
+    let RR := fresh "RR" in
+    pose proof (trans_C_addr α C x) as RR;
+    rewrite ADDR in RR;
+    assert (In (trans_v α v) (aread (trans_m α m) (α addr)));
+    first [rewrite trans_m_aread;
+      exists addr; exists v;
+      symmetry in ACCESS; eauto|ss; eauto]
+  | ACCESS : ctx_M ?C ?M = Some ?CM |- _ =>
+    pose proof (trans_C_ctx_M C α M CM ACCESS); ss; eauto
+  end;
+  repeat match goal with
+  | H : {| (Cf ?e ?C ?m ?t) ~> (Rs ?V ?m' ?t') |} |- _ =>
+    lazymatch goal with
+    | _ : leb t t' = true |- _ => fail
+    | _ =>
+      let INC := fresh "INC" in
+      let BD := fresh "BD" in
+      apply time_increase in H as INC;
+      apply time_bound in H as BD;
+      try solve [ss; eauto]
+    end
+  end;
+  try match goal with
+  | |- {| _ ~#> _ |} =>
+    try exploit IHEVAL1; eauto;
+    try exploit IHEVAL2; eauto;
+    try exploit IHEVAL3; eauto;
+    ii; ss;
+    try rewrite trans_m_update in *;
+    try rewrite PRES in *; des; eauto
+  end; ss; des;
+  try solve [split; eauto using relax_ctx_bound];
+  try match goal with
+  | |- context [tick _ _ ?t _ _] =>
+    split; try (apply time_bound_tick; assumption);
+    red; ii; ss; des; clarify;
+    try match goal with
+    | _ => apply tick_lt
+    | H : supp_C ?C_f _, BD : time_bound_C ?C_f _ |- _ =>
+      apply BD in H; eapply relax_p_bound;
+      first [eassumption | lebt t]
+    end
+  | _ => split; first [assumption | red; ii; ss; des; clarify]
+  end;
+  match goal with
+  | BD : time_bound_C ?C _, _ : supp_C ?C _ |- _ =>
+    solve [apply BD; eauto]
+  | BD : time_bound_C ?C _, H : supp_C ?C _ |- _ =>
+    apply BD in H;
+    solve [eapply relax_p_bound; eassumption]
+  | _ => apply time_bound in EVAL2; ss; des;
+    try match goal with
+    | BD : time_bound_v ?v _, H : supp_v ?v _ |- _ =>
+      destruct v; ss; apply BD in H;
+      eapply relax_p_bound; first [eassumption | apply tick_lt]
+    | BD : time_bound_m ?m _, H : supp_m ?m _ |- _ =>
+      apply BD in H;
+      eapply relax_p_bound; first [eassumption | apply tick_lt]
+    | _ => solve [split; eauto using relax_ctx_bound]
+    end
+  end.
+Qed.
